We first consider the continuous time gradient flow.
The key idea is to consider the following auxiliary ODEs\begin{align*}
\frac{d\widetilde{\mat{W}}(t)}{dt} = &- \mat{Z}(0) \left(\tilde{\vect{u}}(t)-\vect{y}\right) \text{ with } \widetilde{\mat{W}} = \mat{W}(0) \\
\frac{d\tilde{\vect{u}}(t)}{dt} = &- \mat{H}(0)\left(\tilde{\vect{u}}(t)-\vect{y}\right) \text{ and }\tilde{\vect{u}}(0) = \vect{u}(0).
\end{align*} 

Note $\widetilde{\mat{W}}(t)$ is the desired ODE, so we want to bound $\mat{W}-\widetilde{\mat{W}}(t)$.
\begin{lem}\label{lem:gf_optimization}
With high probability over initialization, we have for all $t\ge 0$\begin{align*}
	\norm{\mat{W}(t)-\widetilde{\mat{W}}(t)}_F \le \frac{\poly(n,1/\lambda_0,\log m)}{\sqrt{m}}.
\end{align*}
\end{lem}



Also note, both $\vect{u}(t)-\tilde{\vect{u}}(t)$ will converge to $\vect{y}$ by the analysis in \cite{du2018provably}.
We can compute \begin{align*}
&\frac{d \left(\mat{W}(t)-\widetilde{\mat{W}}(t)\right)}{dt}\\
= &-\mat{Z}(t)(\vect{u}(t)-\vect{y}) + \mat{Z}(0)\left(\tilde{\vect{u}}(t)-\vect{y}\right) \\
= &\left(\mat{Z}(0)-\mat{Z}(t)\right)\left(\vect{u}(t)-\vect{y}\right) + \mat{Z}(0)\left(\tilde{\vect{u}}(t)-\vect{u}(t)\right).
\end{align*}
For the first term, recall in \cite{du2018provably}, they showed for all $t >0$ \begin{align*}
	\norm{\mat{Z}(t) - \mat{Z}(0)}_2 = \frac{\poly(n,1/\lambda_0)}{\sqrt{m}}.
\end{align*}
Therefore we can bound \begin{align*}
	\int \norm{\left(\mat{Z}(0)-\mat{Z}(t)\right)\left(\vect{u}(t)-\vect{y}\right) }_F dt \le \frac{\poly(n,1/\lambda_0)}{\sqrt{m}} \int \norm{\tilde{\vect{u}}(t)-\vect{y}}_2 dt= \frac{\poly(n,1/\lambda_0)}{\sqrt{m}}.
\end{align*}
For the second term, we thus need to bound\begin{align}
\int_{t=0}^{\infty}\norm{\tilde{\vect{u}}(t)-\vect{u}(t)}_2 dt. \label{eqn:u_tilde_u}
\end{align}
To bound Equation~\eqref{eqn:u_tilde_u}, we observe that $\tilde{\vect{u}}(t) \rightarrow \vect{y}$ and $\vect{u}(t) \rightarrow \vect{y}$.
Therefore, we can choose some $t_0$ such that \begin{align*}
\int_{t_0}^\infty\norm{\vect{\tilde{u}}(t)-\vect{u}(t)}_2 dt \le \int_{t_0}^\infty(\norm{\vect{\tilde{u}}(t)-\vect{y}}_2  + \norm{\vect{y}-\vect{u}(t)}_2 )dt
\end{align*}
Note if we choose $t_0 = \frac{C}{\lambda_0}\left(\frac{m\lambda_0}{n}\right)$ so that \begin{align*}
\int_{t_0}^\infty\norm{\vect{\tilde{u}}(t)-\vect{u}(t)}_2 dt \le \frac{2\norm{\vect{u}(t)-\vect{y}}_2}{\lambda_0} \le \frac{\poly(n,1/\lambda_0)}{\sqrt{m}}.
\end{align*}
Thus it suffices to bound \begin{align*}
	\int_{t=0}^{t_0}\norm{\tilde{\vect{u}}(t)-\vect{u}(t)}_2 dt \le t_0 \max_{0\le t\le t_0} \norm{\tilde{\vect{u}}(t)-\vect{u}(t)}_2.
\end{align*}
First observe that \[
 \norm{\tilde{\vect{u}}(t)-\vect{u}(t)}_2 \le \int_{\tau = 0}^t \norm{\frac{d\left(\tilde{\vect{u}}(\tau)-\vect{u}(\tau)\right)}{d \tau}}_2 d\tau.
 \]
 Note \begin{align*}
 &\frac{d \left(\tilde{\vect{u}}(t)-\vect{u}(t)\right)}{dt} \\
 = &-\mat{H}(0)\left(\tilde{\vect{u}}(t)-\vect{y}\right) + \mat{H}(t)\left(\vect{u}(t)-\vect{y}\right) \\
 = &  -\mat{H}(0)\left(\tilde{\vect{u}}(t)-\vect{u}(t)\right) + \left(\vect{u}(t)-\vect{y}\right)\left(\mat{H}(t)-\mat{H}(0)\right).
 \end{align*}
Since $\mat{H}(0)$ is positive semidefinite, $-\mat{H}(0)\left(\tilde{\vect{u}}(t)-\vect{u}(t)\right) $ term only makes $\norm{\tilde{\vect{u}}(t)-\vect{u}(t)}_2$ smaller.
Therefore, we have \begin{align*}
\norm{\tilde{\vect{u}}(t)-\vect{u}(t)}_2 \le &\int_{\tau =0}^t \norm{\vect{u}(\tau)-\vect{y}}_2 \norm{\mat{H}(t)-\mat{H}(0)}_2 \\
\le & t\norm{\vect{u}(0)-\vect{y}}_2 \frac{\poly(n,1/\lambda_0)}{\sqrt{m}} = \frac{t\poly(n,1/\lambda_0)}{\sqrt{m}} .
\end{align*}
Therefore, we have \begin{align*}
	\int_{t=0}^{t_0}\norm{\tilde{\vect{u}}(t)-\vect{u}(t)}_2 dt \le t_0 \max_{0\le t\le t_0} \norm{\tilde{\vect{u}}(t)-\vect{u}(t)}_2 \le t_0^2 \frac{\poly(n,1/\lambda_0)}{\sqrt{m}} \le \frac{\poly(n,1/\lambda_0,\log(m))}{\sqrt{m}}.
\end{align*}
\qed